Cellio example update

examples/cellio/CellioAll.v
@@ -10,20 +10,20 @@ Module CellioAll. Section CellioAll.
   Local Instance Σ : GRA := ##[invΣ; Γ].
   Variable foo: Any.t -> itree hmodE Any.t.
   Local Definition smod_src : SMod.t := MainA.Mod ☆ CellioA.Mod ☆ InputA.Mod ☆ (FooA.Mod foo).
-  Local Definition ginv : Sk.t → invspec := λ _ _, True%I.
-  Local Definition stb : Sk.t → string → option fspec := stb_global smod_src.
+  Local Definition ginv : invspec := λ _, True%I.
+  Local Definition spc : string → option fspec := spc_global smod_src.
   Local Definition mod_cancel : HMod.t := SModCancel.to_hmod smod_src.
-  Local Definition mod_src : HMod.t := SMod.to_hmod ginv stb smod_src.
-  Local Definition mod_tgt : HMod.t := MainI.t ★ CellioI.t ★ (InputA.t ginv stb) ★ (FooA.t foo ginv stb).
+  Local Definition mod_src : HMod.t := SMod.to_hmod ginv spc smod_src.
+  Local Definition mod_tgt : HMod.t := MainI.t ★ CellioI.t ★ (InputA.t ginv spc) ★ (FooA.t foo ginv spc).
 
   Local Definition main_fsp : fspec := fspec_trivial.
-  Local Definition init_cond : Sk.t → iProp Σ := MainA.InitCond ∗∗ CellioA.InitCond ∗∗ InputA.InitCond ∗∗ FooA.InitCond.
-  Local Definition skeleton : Sk.t := Sk.add CellioSK.t MainSK.t.
+  Local Definition init_cond : iProp Σ := MainA.InitCond ∗ CellioA.InitCond ∗ InputA.InitCond ∗ FooA.InitCond.
+  (* Local Definition genv : GEnv.t := GEnv.add CellioGEnv.t MainGEnv.t. *)
 
   (* Apply cancellation to linked spec module *)
   Lemma cancel_src :
-    refines (mod_cancel, init_cond ∗∗ (λ _, main_fsp.(precond) 0 tt tt↑ tt↑)) 
-            ((mod_src, init_cond) : HMod.modc).
+    refines (mod_cancel, (init_cond ∗ main_fsp.(precond) 0 tt tt↑ tt↑)%I) 
+            (mod_src, init_cond).
   Proof.
     eapply cancellation; try by econs.
     i. iIntros "%POST". iPureIntro.
@@ -31,14 +31,14 @@ Module CellioAll. Section CellioAll.
   Qed.
 
   (* Refinement between spec/impl of whole program (linked module) *)
-  Lemma src_tgt : refines (mod_src, init_cond) (mod_tgt, const(emp)%I).
+  Lemma src_tgt : refines (mod_src, init_cond) (mod_tgt, emp%I).
   Proof.
     (* consider identical modules in src/tgt as context (InputA, FooA) *)
     eapply ctxr_refines.
-    rewrite -[(_, const (emp%I))]hmod_addc_empty_r /init_cond -!hmod_addc_assoc.
+    rewrite -[(_, emp%I)]hmod_addc_empty_r /init_cond -!hmod_addc_assoc.
     rewrite /mod_src /mod_tgt !add_interp_comm -!hmod_add_assoc /FooA.t.
     unseal CRIS. eapply ctxr_frameR, ctxr_cond_frameR.
-    rewrite -[(_, const (emp%I))]hmod_addc_empty_r /InputA.t.
+    rewrite -[(_, emp%I)]hmod_addc_empty_r /InputA.t.
     unseal CRIS. eapply ctxr_frameR, ctxr_cond_frameR.
     (* solve by transitivity:
       MainI ★ CellioI ⊆ MainI ★ CellioA ⊆ MainA ★ CellioA 
@@ -47,29 +47,29 @@ Module CellioAll. Section CellioAll.
     {
       (* MainI ★ CellioA ⊆ MainA ★ CellioA *)
       rewrite -[(SMod.to_hmod _ _ MainA.Mod)](Seal.sealing_eq CRIS) -[(SMod.to_hmod _ _ CellioA.Mod)](Seal.sealing_eq CRIS).
-      instantiate (1:= (MainI.t ★ (CellioA.t ginv stb), (const(emp%I)) ∗∗ CellioA.InitCond)).
+      instantiate (1:= (MainI.t ★ (CellioA.t ginv spc), (emp ∗ CellioA.InitCond)%I)).
       eapply ctxr_cond_frameR, main_adequacy, MainIA.sim.
       {
-        i. rewrite /FooAS.Stb. unseal CRIS. econs; first prove_nodup.
-        ii; rewrite -FIND /stb /stb_global /smod_src //=. des_ifs; ss; des_ifs.
+        i. rewrite /FooAS.Spc. unseal CRIS. econs; first prove_nodup.
+        ii; rewrite -FIND /spc /spc_global /smod_src //=. des_ifs; ss; des_ifs.
       }
       {
-        i. rewrite /InputAS.Stb. unseal CRIS. econs; first prove_nodup.
-        ii; rewrite -FIND /stb /stb_global /smod_src //=. des_ifs; ss; des_ifs.
+        i. rewrite /InputAS.Spc. unseal CRIS. econs; first prove_nodup.
+        ii; rewrite -FIND /spc /spc_global /smod_src //=. des_ifs; ss; des_ifs.
       }
     }
     (* MainI ★ CellioI ⊆ MainI ★ CellioA 
       by CellioI ⊆ctx CellioA *)
-    rewrite -[(_, const (emp%I))]hmod_addc_empty_r.
+    rewrite -[(_, emp%I)]hmod_addc_empty_r.
     eapply ctxr_frameL, ctxr_cond_frameL, main_adequacy, CellioIA.sim. 
-    i. rewrite /InputAS.Stb. unseal CRIS. econs; first prove_nodup.
-    ii; rewrite -FIND /stb /stb_global /smod_src //=.
+    i. rewrite /InputAS.Spc. unseal CRIS. econs; first prove_nodup.
+    ii; rewrite -FIND /spc /spc_global /smod_src //=.
     des_ifs; ss; des_ifs.
   Qed.
 
   Lemma cancel_tgt :
-    refines (mod_cancel, init_cond ∗∗ (λ _, main_fsp.(precond) 0 tt tt↑ tt↑))
-            (mod_tgt, const(emp)%I).
+    refines (mod_cancel, (init_cond ∗ main_fsp.(precond) 0 tt tt↑ tt↑)%I)
+            (mod_tgt, emp%I).
   Proof.
     etrans.
     { eapply cancel_src. }
@@ -86,16 +86,14 @@ Module CellioAll. Section CellioAll.
   Qed.
 
   Theorem behavioral_refinement :
-    ∃ target_resource, refines_modsem
-      (HModSem.to_mod ((HMod.modsem mod_cancel) skeleton) initial_resource)
-      (HModSem.to_mod ((HMod.modsem mod_tgt) skeleton) target_resource).
+    ∃ target_resource, refines_mod
+      (HMod.to_mod mod_cancel initial_resource)
+      (HMod.to_mod mod_tgt target_resource).
   Proof.
     move: (cancel_tgt)=>H; rewrite /refines in H; des; ss.
-    destruct (REF skeleton initial_resource).
-    { rewrite /CellioI.t /MainI.t /InputA.t /FooA.t /skeleton; unseal CRIS; ss. }
-    { rewrite /skeleton /CellioSK.t /MainSK.t; ss; econs; ii; ss; des; ss; prove_nodup. }
+    destruct (H initial_resource).
     { apply initial_resource_valid. }
-    { iIntros "I"; rewrite /init_cond /CellioA.InitCond /MainA.InitCond /InputA.InitCond /FooA.InitCond /HMod.addc.
+    { iIntros "I"; rewrite /init_cond /CellioA.InitCond /MainA.InitCond /InputA.InitCond /FooA.InitCond.
       rewrite /precond /= /CellioA.auth 
        own.Own_eq own.own_eq /own.Own_def /own.own_def. 
       iDestruct "I" as "[[[_ I] _] _]"; iFrame. 
